---
title: "EX2"
author: "roi hezkiyahu"
date: "11 3 2022"
output: html_document
---

```{r setup, include=FALSE}
knitr::opts_chunk$set(echo = TRUE)
```

#Q.1

![](Q1.png)

#Q.2

![](Q2.png)

**1**

$$
y = ax +b +\varepsilon\\
x_i = x_j\quad \forall i,j\\
h_{ii} = \frac{1}{n} + \frac{(x_i - \bar{x})^2}{\sum_{i=1}^n(x_j-\bar{x})^2}\\
x_i-\bar{x} = d \Rightarrow h_{ii} = \frac{1}{n} + \frac{d^2}{nd^2} = \frac{2}{n}
$$

**2**

*w.l.o.g we can assume i = 1 is the different x*

$$
x_j = w \quad \forall j>1\\
\bar{x} = \frac{x_1}{n} + \frac{(n-1)}{n}w\\
x_1 -\bar{x} = x_1 -  \frac{x_1}{n} - \frac{(n-1)}{n}w = \frac{(n-1)(w-x_1)}{n}\\
x_j -\bar{x} = w -  \frac{x_1}{n} - \frac{(n-1)}{n}w = \frac{(w-x_1)}{n}\\
\sum_{j=1}^n(x_j -\bar{x})^2 = (x_1 -\bar{x})^2 + (n-1)(w -\bar{x})^2 = (\frac{(n-1)(w-x_1)}{n})^2 + (n-1)\frac{(w-x_1)^2}{n^2} = \frac{[(n-1)^2-(n-1)](w-x_1)^2}{n^2} = \frac{(n-1)(w-x_1)^2}{n}\\
h_{11} = \frac{1}{n} +  \frac{(x_1 -\bar{x})^2}{\sum_{j=1}^n(x_j -\bar{x})^2} = \frac{1}{n} + \frac{n-1}{n} = 1\\
h_{jj} = \frac{1}{n} +  \frac{(x_j -\bar{x})^2}{\sum_{k=1}^n(x_k -\bar{x})^2} = \frac{1}{n} + \frac{(\frac{(w-x_1)}{n})^2}{\frac{(n-1)(w-x_1)^2}{n}}  =\frac{1}{n} + \frac{1}{n(n-1)} = \frac{1}{n-1}
$$

#Q.3

![](Q3.png)


#Q.4

![](Q4.png)





